## Sum contrast

::: columns

:::: pull-left

$$\begin{aligned}
{H_0}_1: \overbrace{\mu_1}^{\text{低頻度語への反応時間}} & = \overbrace{\frac{\mu_1 + \mu_2 + \mu_3}{3}}^{全体平均}\\
\Leftrightarrow \mu_1 & = \frac{1}{3}\mu_1 + \frac{1}{3}\mu_2 + \frac{1}{3}\mu_3 \\
\Leftrightarrow \frac{2}{3}\mu_1 - \frac{1}{3}\mu_2 - \frac{1}{3}\mu_3 & = 0\\
(\underbrace{\frac{2}{3}}_{\mu_1\text{への重み}}\mu_1) + (\underbrace{-\frac{1}{3}}_{\mu_2\text{への重み}}\mu_2) + (\underbrace{-\frac{1}{3}}_{\mu_3\text{への重み}}\mu_3) & = 0
\end{aligned}$$

::::

:::: pull-right

$$\begin{aligned}
{H_0}_1: \overbrace{\mu_2}^{\text{中頻度語への反応時間}} & = \overbrace{\frac{\mu_1 + \mu_2 + \mu_3}{3}}^{全体平均}\\
\Leftrightarrow \mu_2 & = \frac{1}{3}\mu_1 + \frac{1}{3}\mu_2 + \frac{1}{3}\mu_3 \\
\Leftrightarrow -\frac{1}{3}\mu_1 + \frac{2}{3}\mu_2 - \frac{1}{3}\mu_3 & = 0\\
(\underbrace{-\frac{1}{3}}_{\mu_1\text{への重み}}\mu_1) + (\underbrace{\frac{2}{3}}_{\mu_2\text{への重み}}\mu_2) + (\underbrace{-\frac{1}{3}}_{\mu_3\text{への重み}}\mu_3) & = 0
\end{aligned}$$

::::

:::

---
